I broke 5.4 to smaller lemmas so there wouldn't be any 'forall' commands in the 5.4 implament. The smaller lemmas still have some errors (6 in total). The dummy4allrange might be a bit tricky (3 diffrent kinds of errors). As for the dummy 6 to SliceRefinement lemma there is an error on the step between dummy3 and the 'forall..' in the theory the same as one of the errors we can also see in the dummy4allRange (the same goes for CoDummy6 and CoSliceRefinement lemma).
Once the 5.4 is complete all that is left is 5.3Right and 5.1 (not counting the 'assume's).

I am thinking about beraking 5.1 the same as we have done in 5.3

SliceRefinements.dfy
@@ -292,8 +292,9 @@ function method varsInExps(exps: seq<Expression>): set<Variable>
 	if exps == [] then {} else exps[0].1+varsInExps(exps[1..])
 }
 
-
-// *** Definitions ***
+//============================================================
+//					*** Definitions ***
+//============================================================
 
 predicate EquivalentPredicates(P1: Predicate, P2: Predicate) reads *
 {
@@ -357,9 +358,9 @@ requires Valid(S1)
 requires Valid(S2)
 ensures CoSliceRefinement(S1, S2, V) <==> (forall P: Predicate,s: State :: (vars(P) !! V) ==> ((wp(S1,P).0(s) ==> wp(S2,P).0(s))))
 
-
-// *** Predicate Operators ***
-
+//============================================================
+//					*** Predicate Operators ***
+//============================================================
 function AND(P1: Predicate,P2: Predicate): Predicate
 {
 	((s: State) reads * requires P1.0.requires(s) && P2.0.requires(s) => P1.0(s) && P2.0(s),P1.1 + P2.1)
@@ -427,8 +428,9 @@ requires Valid(S)
 requires Valid(Sco)
 ensures (forall s: State, v: Variable :: v in V && v in s ==> var P:= (((s1: State) reads *  => v in s1 && s1[v] == s[v]),{v}); (wp(S,P).0(s) ==> wp(Sco,P).0(s)))
 
-// *** RE1-5 ***
-
+//============================================================
+//					*** RE1-RE5 ***
+//============================================================
 function VarsOfPredicateSet(W: set<Predicate>): set<Variable>
 {
 	if W == {} then {} else var w :| w in W; w.1 + VarsOfPredicateSet(W-{w})
@@ -616,7 +618,7 @@ ensures EquivalentPredicates(wp(S,P), AND(P, wp(S,ConstantPredicate(true))))
 			wp(S0,P).0(s);
 			== {assert vars(P) !! def(S0) by {assert def(S) !! vars(P);assert setOf(L) !! vars(P) by {LocalDecStrangers(S,P); }}RE3(S0,P);/**/}
 			AND(P, wp(S0,ConstantPredicate(true))).0(s);
-			== //{ vars(ConstantPrdicate(true)) = XX;} //TODO 26/11/16: pharse this
+			== {} 
 			AND(P, wp(S,ConstantPredicate(true))).0(s); 
 		}
 		}
@@ -662,7 +664,9 @@ lemma RE5(S: Statement)
 }
 */
 
-// *** THEOREMS ***
+//============================================================
+//					*** THEOREMS ***
+//============================================================
 
 lemma {:verify true} AbsorptionOfTermination3_14(P: Predicate,S: Statement)
 	requires Valid(S)
@@ -715,6 +719,7 @@ ensures (forall P: Predicate, s:State :: vars(P) !! V ==> ((wp(S,P).0(s) ==> wp(
 
 
 /*TODO : Complete 3 err*/
+// try to break it into 2
 lemma {:verify false} Theorem_5_1 (S: Statement, SV: Statement, V: set<Variable>)
 requires Valid(S)
 requires Valid(SV)
@@ -738,21 +743,35 @@ ensures SliceRefinement(S,SV,V) <==> (forall s: State :: ((wp(S,ConstantPredicat
 			assert EquivalentPredicates(P4,P5);
 			Leibniz2(wp, P4,P5, S);}
 		wp(S,(((s1: State) reads * requires P.0.requires(s1) => exists p: State :: P.0.requires(p) && P.0(p) && P2(p).0(s1)), P.1)).0(s);
-		== { assert EquivalentPredicates(wp(S,(((s1: State) reads * requires P.0.requires(s1) => exists p: State :: P.0.requires(p) && P.0(p) && P2(p).0(s1)), P.1)),P3) by { RE1(S,{P/*2(p)*/});}} 
+		== { assume EquivalentPredicates(wp(S,(((s1: State) reads * requires P.0.requires(s1) => exists p: State :: P.0.requires(p) && P.0(p) && P2(p).0(s1)), P.1)),P3) /*by { RE1(S,{P/*2(p)*/});}*/;} 
 		//(((s1: State) reads * requires P.0.requires(s1) => exists p: State :: P.0.requires(p) && P.0(p) && wp.requires(S,P2(p)) && (wp(S,P2(p)).0(s1))), P.1).0(s);
 		//=={}                                                                                              
-		  wp(S,P3).0(s);
+		P3.0(s);
 		== {}
 		(exists p: State :: P.0.requires(p) && P.0(p) && wp(S,((s0:State)=>(forall v: Variable :: v in V ==> v in s0 && v in p && s0[v] == p[v]),P.1)).0(s));
 		}
 	}
 }
 
+
+predicate dummy3(S: Statement, SV: Statement, V: set<Variable>)
+reads *
+requires Valid(S)
+requires Valid(SV)
+{
+	(((forall s: State :: ((wp(S,ConstantPredicate(true)).0(s) ==> wp(SV,ConstantPredicate(true)).0(s)))) && (forall s: State, v: Variable :: v in (def(S)+def(SV)-V) && v in s ==> var P:= (((s1: State) reads *  => v in s1 && s1[v] == s[v]),{v}); (wp(S,P).0(s) ==> wp(SV,P).0(s)))))
+}
+
+lemma dummy3Lemma(S: Statement, SV: Statement, V: set<Variable>)
+requires Valid(S)
+requires Valid(SV)
+ensures dummy3(S,SV,V) <==> (((forall s: State :: ((wp(S,ConstantPredicate(true)).0(s) ==> wp(SV,ConstantPredicate(true)).0(s)))) && (forall s: State, v: Variable :: v in (def(S)+def(SV)-V) && v in s ==> var P:= (((s1: State) reads *  => v in s1 && s1[v] == s[v]),{v}); (wp(S,P).0(s) ==> wp(SV,P).0(s)))))
+
+
 lemma {:verify true} Corollary_5_2 (S: Statement, SV: Statement, V: set<Variable>)
 requires Valid(S)
 requires Valid(SV)
-ensures (CoSliceRefinement(S,SV,V)) ==> (((forall s: State :: ((wp(S,ConstantPredicate(true)).0(s) ==> wp(SV,ConstantPredicate(true)).0(s)))) && (forall s: State, v: Variable :: v in (def(S)+def(SV)-V) && v in s ==> var P:= (((s1: State) reads *  => v in s1 && s1[v] == s[v]),{v}); (wp(S,P).0(s) ==> wp(SV,P).0(s)))))
-ensures (CoSliceRefinement(S,SV,V)) <== (((forall s: State :: ((wp(S,ConstantPredicate(true)).0(s) ==> wp(SV,ConstantPredicate(true)).0(s)))) && (forall s: State, v: Variable :: v in (def(S)+def(SV)-V) && v in s ==> var P:= (((s1: State) reads *  => v in s1 && s1[v] == s[v]),{v}); (wp(S,P).0(s) ==> wp(SV,P).0(s)))))
+ensures (CoSliceRefinement(S,SV,V)) <==> dummy3(S,SV,V)
 {
 	calc {
 	CoSliceRefinement(S,SV,V);
@@ -760,6 +779,8 @@ ensures (CoSliceRefinement(S,SV,V)) <== (((forall s: State :: ((wp(S,ConstantPre
 	SliceRefinement(S,SV,(def(S) + def(SV)) - V);
 	== {Theorem_5_1(S,SV,(def(S) + def(SV)) - V);}
 	((forall s:State :: ((wp(S,ConstantPredicate(true)).0(s) ==> wp(SV,ConstantPredicate(true)).0(s)))) && (forall s: State, v: Variable :: v in (def(S)+def(SV)-V) && v in s ==> var P:= (((s1: State) reads *  => v in s1 && s1[v] == s[v]),{v}); (wp(S,P).0(s) ==> wp(SV,P).0(s))));
+	== {dummy3Lemma(S,SV,V);}
+	dummy3(S,SV,V);
 	}
 }
 
@@ -814,8 +835,129 @@ ensures CoSliceRefinement(S,SV,V) <== SliceRefinement(S,SV,CoV)
 	}
 }
 
+predicate dummy4(S: Statement, SV: Statement, V: set<Variable>)
+reads *
+requires Valid(S)
+requires Valid(SV)
+{
+	(forall s: State :: ((wp(S,ConstantPredicate(true)).0(s) ==> wp(SV,ConstantPredicate(true)).0(s)))) && (forall s: State ,v: Variable ,P: Predicate :: v in (V+def(S)+def(SV)) && v in P.1 ==> (wp(S,P).0(s) ==> wp(SV,P).0(s)))
+}
 
-/*TODO : Complete 4 err*/
+lemma dummy4Lemma(S: Statement, SV: Statement, V: set<Variable>)
+requires Valid(S)
+requires Valid(SV)
+ensures dummy4(S,SV,V) <==> (forall s: State :: ((wp(S,ConstantPredicate(true)).0(s) ==> wp(SV,ConstantPredicate(true)).0(s)))) && (forall s: State ,v: Variable ,P: Predicate :: v in (V+def(S)+def(SV)) && v in P.1 ==> (wp(S,P).0(s) ==> wp(SV,P).0(s)))
+
+// TODO: complete 4 errr
+lemma {:verify false} dummy4AllRange(S: Statement, SV: Statement, V: set<Variable>)
+requires Valid(S)
+requires Valid(SV)
+ensures dummy3(S,SV,{}) <==>  dummy4(S,SV,V)
+{
+	forall s: State, v: Variable  {
+	calc {
+	dummy3(S,SV,{});
+	== {dummy3Lemma(S,SV,{});}
+	(((forall s: State :: ((wp(S,ConstantPredicate(true)).0(s) ==> wp(SV,ConstantPredicate(true)).0(s)))) && (forall s: State, v: Variable :: v in (def(S)+def(SV)-{}) && v in s ==> var P:= (((s1: State) reads *  => v in s1 && s1[v] == s[v]),{v}); (wp(S,P).0(s) ==> wp(SV,P).0(s)))));
+	== {}
+	((forall s: State :: ((wp(S,ConstantPredicate(true)).0(s) ==> wp(SV,ConstantPredicate(true)).0(s)))) && (forall s: State ,v: Variable ,P: Predicate :: v in (def(S)+def(SV)-{}) && v in P.1 ==> (wp(S,P).0(s) ==> wp(SV,P).0(s))));
+	== {var P:=  (((s1: State) reads *  =>  v in (def(S)+def(SV)-{}) && v in s && v in s1 && s1[v] == s[v]),{v});Corollary_5_5(S, SV,P);}
+	(forall s: State :: ((wp(S,ConstantPredicate(true)).0(s) ==> wp(SV,ConstantPredicate(true)).0(s)))) && (forall s: State ,v: Variable ,P: Predicate :: v in (V+def(S)+def(SV)) && v in P.1 ==> (wp(S,P).0(s) ==> wp(SV,P).0(s)));
+	== {dummy4Lemma(S,SV,V);}
+	dummy4(S,SV,V);
+	}
+	}
+}
+
+predicate dummy5(S: Statement, SV: Statement, V: set<Variable>)
+reads *
+requires Valid(S)
+requires Valid(SV)
+{
+	(forall s: State :: ((wp(S,ConstantPredicate(true)).0(s) ==> wp(SV,ConstantPredicate(true)).0(s)))) && (forall s: State ,v: Variable ,P: Predicate :: v in (V) && v in P.1 ==> (wp(S,P).0(s) ==> wp(SV,P).0(s))) && (forall s: State ,v: Variable ,P: Predicate :: v in ((def(S)+def(SV))-V) && v in P.1 ==> (wp(S,P).0(s) ==> wp(SV,P).0(s)))
+}
+
+lemma dummy5Lemma(S: Statement, SV: Statement, V: set<Variable>)
+requires Valid(S)
+requires Valid(SV)
+ensures dummy5(S,SV,V) <==> (forall s: State :: ((wp(S,ConstantPredicate(true)).0(s) ==> wp(SV,ConstantPredicate(true)).0(s)))) && (forall s: State ,v: Variable ,P: Predicate :: v in (V) && v in P.1 ==> (wp(S,P).0(s) ==> wp(SV,P).0(s))) && (forall s: State ,v: Variable ,P: Predicate :: v in ((def(S)+def(SV))-V) && v in P.1 ==> (wp(S,P).0(s) ==> wp(SV,P).0(s)))
+
+lemma dummy5dummy6Lemma(S: Statement, SV: Statement, V: set<Variable>,CoV: set<Variable>)
+requires Valid(S)
+requires Valid(SV)
+requires CoV == (def(S) + def(SV)) - V
+ensures dummy5(S,SV,V) <==> dummy6(S,SV,V,CoV) && CoDummy6(S,SV,V,CoV)
+
+
+predicate dummy6(S: Statement, SV: Statement, V: set<Variable>,CoV: set<Variable>)
+reads *
+requires Valid(S)
+requires Valid(SV)
+requires CoV == (def(S) + def(SV)) - V
+{
+	(forall s: State :: ((wp(S,ConstantPredicate(true)).0(s) ==> wp(SV,ConstantPredicate(true)).0(s)))) && (forall s: State ,v: Variable ,P: Predicate :: v in (V) && v in P.1 ==> (wp(S,P).0(s) ==> wp(SV,P).0(s)))
+}
+
+predicate CoDummy6(S: Statement, SV: Statement, V: set<Variable>,CoV: set<Variable>)
+reads *
+requires Valid(S)
+requires Valid(SV)
+requires CoV == (def(S) + def(SV)) - V
+{
+	(forall s: State :: ((wp(S,ConstantPredicate(true)).0(s) ==> wp(SV,ConstantPredicate(true)).0(s)))) && (forall s: State ,v: Variable ,P: Predicate :: v in (CoV) && v in P.1 ==> (wp(S,P).0(s) ==> wp(SV,P).0(s)))
+}
+
+
+lemma dummy6Lemma(S: Statement, SV: Statement, V: set<Variable>,CoV: set<Variable>)
+requires Valid(S)
+requires Valid(SV)
+requires CoV == (def(S) + def(SV)) - V
+ensures dummy6(S,SV,V,CoV) <==> (forall s: State :: ((wp(S,ConstantPredicate(true)).0(s) ==> wp(SV,ConstantPredicate(true)).0(s)))) && (forall s: State ,v: Variable ,P: Predicate :: v in (V) && v in P.1 ==> (wp(S,P).0(s) ==> wp(SV,P).0(s))) 
+
+lemma CoDummy6Lemma(S: Statement, SV: Statement, V: set<Variable>,CoV: set<Variable>)
+requires Valid(S)
+requires Valid(SV)
+requires CoV == (def(S) + def(SV)) - V
+ensures CoDummy6(S,SV,V,CoV) <==> (forall s: State :: ((wp(S,ConstantPredicate(true)).0(s) ==> wp(SV,ConstantPredicate(true)).0(s)))) && (forall s: State ,v: Variable ,P: Predicate :: v in (CoV) && v in P.1 ==> (wp(S,P).0(s) ==> wp(SV,P).0(s))) 
+
+// TODO: Complete 1 err
+lemma {:verify false} CoDummy6CoSliceRefinementLemma(S: Statement, SV: Statement, V: set<Variable>,CoV: set<Variable>)
+requires Valid(S)
+requires Valid(SV)
+requires CoV == (def(S)+def(SV))-V
+ensures CoSliceRefinement(S,SV,V) <==> CoDummy6(S,SV,V,CoV)
+{
+	calc {
+		CoDummy6(S,SV,V,CoV);
+		== {CoDummy6Lemma(S,SV,V,CoV);}
+		(forall s: State :: ((wp(S,ConstantPredicate(true)).0(s) ==> wp(SV,ConstantPredicate(true)).0(s)))) && (forall s: State ,v: Variable ,P: Predicate :: v in (CoV) && v in P.1 ==> (wp(S,P).0(s) ==> wp(SV,P).0(s)));
+		== {assert CoV == (def(S)+def(SV)-V);}
+		(((forall s: State :: ((wp(S,ConstantPredicate(true)).0(s) ==> wp(SV,ConstantPredicate(true)).0(s)))) && (forall s: State, v: Variable :: v in (def(S)+def(SV)-V) && v in s ==> var P:= (((s1: State) reads *  => v in s1 && s1[v] == s[v]),{v}); (wp(S,P).0(s) ==> wp(SV,P).0(s)))));
+		== {dummy3Lemma(S,SV,V);}
+		dummy3(S,SV,V);
+		== {Corollary_5_2(S,SV,V);}
+		CoSliceRefinement(S,SV,V);
+	}
+}
+
+// TODO: Complete 1 err
+lemma {:verify false} dummy6SliceRefinementLemma(S: Statement, SV: Statement, V: set<Variable>,CoV: set<Variable>)
+requires Valid(S)
+requires Valid(SV)
+requires CoV == (def(S)+def(SV))-V
+ensures SliceRefinement(S,SV,V) <==> dummy6(S,SV,V,CoV)
+{
+	calc {
+		dummy6(S,SV,V,CoV);
+		=={dummy6Lemma(S,SV,V,CoV);}
+		(forall s: State :: ((wp(S,ConstantPredicate(true)).0(s) ==> wp(SV,ConstantPredicate(true)).0(s)))) && (forall s: State ,v: Variable ,P: Predicate :: v in (V) && v in P.1 ==> (wp(S,P).0(s) ==> wp(SV,P).0(s)));
+		== {}
+		(forall s: State :: ((wp(S,ConstantPredicate(true)).0(s) ==> wp(SV,ConstantPredicate(true)).0(s)))) && (forall s: State, v: Variable :: v in V && v in s ==> var P:= (((s1: State) reads *  => v in s1 && s1[v] == s[v]),{v}); (wp(S,P).0(s) ==> wp(SV,P).0(s)));
+		== {Theorem_5_1(S,SV,V);}
+		SliceRefinement(S,SV,V);
+	}
+}
+
 lemma {:verify true} Corollary_5_4 (S: Statement, T: Statement, V: set<Variable>)
 requires Valid(S)
 requires Valid(T)
@@ -830,7 +972,16 @@ ensures Refinement(S,T) <==> SliceRefinement(S,T,V) && CoSliceRefinement(S,T,V)
 		== {CoSliceRefinementLemma(S,T,{});}
 		CoSliceRefinement(S,T,{});
 		== {Corollary_5_2 (S, T, {});} 
-		((forall s: State :: ((wp(S,ConstantPredicate(true)).0(s) ==> wp(T,ConstantPredicate(true)).0(s)))) 
+		dummy3(S,T,{});
+		== {dummy4AllRange(S,T,V);}
+		dummy4(S,T,V);
+		== {}
+		dummy5(S,T,V);
+		== {}
+		dummy6(S,T,V,(def(S)+def(T))-V) && CoDummy6(S,T,V,(def(S)+def(T))-V);
+		== {dummy6SliceRefinementLemma(S,T,V,(def(S)+def(T))-V);CoDummy6CoSliceRefinementLemma(S,T,V,(def(S)+def(T))-V);}
+		SliceRefinement(S,T,V) && CoSliceRefinement(S,T,V);
+		/*((forall s: State :: ((wp(S,ConstantPredicate(true)).0(s) ==> wp(T,ConstantPredicate(true)).0(s)))) 
 		&& (forall s: State ,v: Variable ,P: Predicate :: v in (def(S)+def(T)-{}) && v in P.1 ==> (wp(S,P).0(s) ==> wp(T,P).0(s))));
 		== {}
 		(forall s: State :: ((wp(S,ConstantPredicate(true)).0(s) ==> wp(T,ConstantPredicate(true)).0(s)))) 
@@ -856,7 +1007,7 @@ ensures Refinement(S,T) <==> SliceRefinement(S,T,V) && CoSliceRefinement(S,T,V)
 		&& ((forall s: State :: ((wp(S,ConstantPredicate(true)).0(s) ==> wp(T,ConstantPredicate(true)).0(s)))) 
 		&& (forall s: State ,v: Variable ,P: Predicate :: v in ((def(S)+def(T))-V) && v in P.1 ==> (wp(S,P).0(s) ==> wp(T,P).0(s))));
 		== {Corollary_5_2(S,T,V);}
-		SliceRefinement(S,T,V) && CoSliceRefinement(S,T,V);
+		SliceRefinement(S,T,V) && CoSliceRefinement(S,T,V);*/
 		}
 }
 
